Main.lean
@@ -1,18 +1,18 @@
 import Bf
 
-open Zen.Train.Bf in
+open Zen.Train.Bf
+
 def main (_args : List String) : IO Unit := do
   for n in [0:30] do
-    let config :=
-        .allOff
-        -- { Rt.Config.allOff with dbg := true }
+    let config := .allOff
+    -- let config := .default
 
-    -- -- stack overflow :/
-    -- let res ←
-    --   Zen.Train.Bf.Std.fibOfInput.evalIOTo! [n] .head! config
-
-    -- no stack overflow :)
+    -- stack overflow :/
     let res ←
-      Zen.Train.Bf.Std.fibOfInput.fastEvalIOTo! [n] .head! config
+      Zen.Train.Bf.Std.fib.evalIOTo! [n] .head! config
+
+    -- -- no stack overflow :)
+    -- let res ←
+    --   Zen.Train.Bf.Std.fib.fastEvalIOTo! [n] .head! config
 
     println! "fib {n} := {res}"
